New minimal start

Flow.v
@@ -8,426 +8,62 @@ Local Open Scope string_scope.
 Local Open Scope Z_scope.
 Local Open Scope list_scope.
 
-Module Flow.
+Module Flow3.
 
-Definition flow : Type := heap -> heap -> Prop.
+Inductive flow : Type :=
+| req : precond -> flow
+| ens : postcond -> flow
+| seq : flow -> flow -> flow
+.
 
-Definition fexists {A: Type} (P: A -> flow) : flow :=
-  fun h1 h2 => exists a: A, P a h1 h2.
+Infix ";;" := seq (at level 80, right associativity).
 
-(* h3 is the part of the heap that is taken away by req,
-   h4 is what is left *)
-Definition freq (P: precond) (k : flow) : flow :=
-  fun h1 h2 => exists h3 h4,
-    h1 = hunion h3 h4 /\ hdisjoint h3 h4 /\ P h3
-    ->
-    k h4 h2.
-
-Definition fens (P: postcond) : flow :=
-  fun h1 h2 => exists h3,
-  exists r, (* TODO *)
-    P r h3 /\ h2 = hunion h1 h3 /\ hdisjoint h1 h3.
-
-Definition fempty : flow := fens (fun r h => True).
-
-Definition fseq (f1 f2 : flow) : flow :=
-  fun h1 h2 => exists h3, f1 h1 h3 /\ f2 h3 h2.
-  (* fun h1 h2 => exists h3, f1 h1 h3 -> f2 h3 h2. *)
-
-Infix ";;" := fseq (at level 80, right associativity).
-
-(* TODO disjunction *)
-
-(* TODO functions *)
-
-(* Definition fn (name : string) : flow :=
-  fun _ => True. *)
+Inductive satisfies : heap -> heap -> flow -> Prop :=
+  | sem_req: forall h3 p h1,
+    (exists h2, h3 = hunion h1 h2 /\ hdisjoint h1 h2 /\ p h2) ->
+    satisfies h3 h1 (req p)
+  | sem_ens: forall h1 h2 h3 q v,
+    h3 = hunion h1 h2 -> hdisjoint h1 h2 ->
+    q v h2 ->
+    satisfies h1 h3 (ens q)
+.
 
 (* forward rules. says how to produce a flow from a program *)
 Inductive forward : com -> flow -> Prop :=
   | fw_skip:
-    forward SKIP fempty
+    forward SKIP (ens (fun v h => True))
   | fw_pure: forall n,
-    forward (PURE n) (fens (fun res => pure (res = n)))
+    forward (PURE n) (ens (fun res => pure (res = n)))
   | fw_get: forall l v, 
     forward (GET l)
-      (freq (contains l v)
-      (fens (fun r => (r = v) //\\ contains l v)))
-
-
-  (* | fw_set: forall f l v, *)
-    (* forward f (SET l v) f *)
-  (* | fw_let: forall f e1 e2, *)
-    (* forward f (LET e1 e2) f *)
-
-  .
-
-(* this axiomatization of the models relation is not needed because of the semantic definitions above *)
-(* Inductive satisfies : heap -> flow -> heap -> Prop :=
-  | m_req: forall h1 h2 p k,
-    satisfies h1 (freq p k) h2
-  | m_ens: forall h1 h2 q,
-    satisfies h1 (fens q) h2
-. *)
-
-(* Example e1 : forall h1 h2, red (PURE 0, h1) (PURE 0, h2).
-intros.
-Qed. *)
-
-
-(* Inductive a : flow -> com -> flow -> Prop := . *)
-
-(* Inductive red: com * heap -> com * heap -> Prop := *)
-
-(* red is a small step relation, soundness eventually needs to be proved for star red *)
-
-(* Ltac inv H := inversion H; clear H; subst. *)
+      (req (contains l v) ;;
+      (ens (fun r => (r = v) //\\ contains l v)))
+.
 
 Definition terminated (c: com) : Prop :=  c = SKIP.
 
 Definition terminates (c1: com) (h1 h2: heap) : Prop :=
   exists c2, star red (c1, h1) (c2, h2) /\ terminated c2.
 
-(* Definition goeswrong (c1: com) (h1: heap) : Prop :=
-  exists c2 h2, star red (c1, h1) (c2, h2) /\ error c2 h2. *)
-
-(* Fixpoint error (c: com) (s: heap) : Prop :=
-  match c with
-  | ASSERT b => beval b s = false
-  | (c1 ;; c2) => error c1 s
-  | _ => False
-  end. *)
-
-
 Theorem soundness : forall f c1 h1 h2 h3,
+  satisfies h1 h3 f ->
   forward c1 f ->
   terminates c1 h1 h2 ->
-  f h1 h3 ->
   h2 = h3.
 Proof.
-admit.
-Admitted.
-
-Theorem soundness0 : forall f c1 c2 h1 h2,
-(* TODO doesn't say anything about stuff that doesn't reduce, like pure *)
-  red (c1, h1) (c2, h2) ->
-  forward c1 f ->
-  f h1 h2.
-Proof.
-  intros f c1 c2 h1 h2 Hr Hf.
-  induction Hf.
-  - inv Hr.
-  - inv Hr.
-  -
-  (* inversion Hr. *)
-  (* assert (fh = fempty). *)
-  inv Hr.
-
-  (* assuming we start in state h2 *)
-  (* the intermediate states in sequencing are also h2 *)
-  (* unfold fseq. *)
-  (* exists h2. *)
-  (* intros hist. *)
-
-  (* now partition the heap into h2 and emp,
-  and assume there is h2[l:=v] *)
-  unfold freq.
-  exists (hsingle l v).
-  exists (hfree l h2).
-  intros [h3 [h4 Hd]].
-  subst.
-  (* h2 is now called h0, and h4 is empty *)
-
-  (* add another empty piece of heap, h3 *)
-  unfold fens.
-  exists (hsingle l v).
-  exists v.
-  subst.
-  split.
-  split; reflexivity.
-  split.
-  + rewrite hunion_comm; auto.
-  + rewrite hdisjoint_sym; auto.
-Qed.
-(* Admitted. *)
-
-End Flow.
-
-Module Flow2.
-
-  Definition flow : Type := heap -> heap -> bool -> Z -> Prop.
-
-  Definition fexists {A: Type} (P: A -> flow) : flow :=
-    fun h1 h2 p r =>
-      exists a: A, P a h1 h2 p r.
-    
-  (* h3 is the part of the heap that is taken away by req,
-    h4 is what is left *)
-  (* Definition freq (P: precond) : flow :=
-    fun h1 h2 p r =>
-        (exists h3 h4, h1 = hunion h3 h4
-          /\ hdisjoint h3 h4
-          /\ P h3 /\ h2 = h4 /\ p = true)
-        \/
-        (forall h3 h4, h1 = hunion h3 h4
-          /\ hdisjoint h3 h4
-          /\ not (P h3) -> p = false). *)
-
-  Definition freq (P: precond) : flow :=
-    fun h1 h2 p r =>
-        (exists h3 h4, h1 = hunion h3 h4
-          /\ hdisjoint h3 h4
-          /\ P h3 -> h2 = h4 /\ p = true)
-        /\
-        (not (exists h3 h4, h1 = hunion h3 h4
-          /\ hdisjoint h3 h4
-          /\ P h3) -> p = false).
-
-  Definition fens (P: postcond) : flow :=
-    fun h1 h2 p r =>
-      exists h3,
-        P r h3
-        /\ h2 = hunion h1 h3
-        /\ hdisjoint h1 h3.
-
-  Definition fempty : flow := fens (fun r h => h = hempty).
-
-  Definition fseq (f1 f2 : flow) : flow :=
-    fun h1 h2 p r =>
-        (exists h3 r1,
-          f1 h1 h3 true r1 /\ f2 h3 h2 p r)
-        \/ f1 h1 h2 false r.
-
-  Infix ";;" := fseq (at level 80, right associativity).
-
-  Example ex_take_put_back : forall x v r, (freq (contains x v) ;; fens (fun r => contains x v)) (hupdate x v hempty) (hupdate x v hempty) true r.
-  Proof.
-    intros.
-    unfold fseq.
-    left.
-    exists hempty. exists 1.
-    split.
-    - unfold freq.
-    left.
-    exists (hupdate x v hempty).
-    exists hempty.
-    split.
-    rewrite <- hunion_comm.
-    rewrite hunion_empty.
-    reflexivity.
-    rewrite hdisjoint_sym.
-    apply hdisjoint_empty.
-    split.
-    HDISJ.
-    split.
-    unfold contains.
-    reflexivity.
-    split; auto.
-    - unfold fens.
-    exists (hupdate x v hempty).
-    repeat split.
-    rewrite hunion_empty.
-    reflexivity.
-    apply hdisjoint_empty.
-  Qed.
-
-  Example ex_vacuous_req : forall x v r, (freq (contains x v)) (hempty) (hupdate x v hempty) false r.
-  Proof.
-    intros.
-    unfold freq.
-    (* taking right branch is easy, but soundness seems difficult as we can always take it *)
-    (* right.
-    intros.
-    reflexivity. *)
-    left.
-    (* cannot prove if i take the left branch *)
-    exists hempty.
-    exists hempty.
-    repeat split.
-    rewrite hunion_empty.
-    reflexivity.
-    apply hdisjoint_empty.
-  Abort.
-
-  Example ex_take : forall x v r, (freq (contains x v)) (hupdate x v hempty) (hempty) false r.
-  Proof.
-    intros.
-    unfold freq.
-    left.
-    exists (hupdate x v hempty).
-    exists hempty.
-    repeat split.
-    rewrite hunion_comm.
-    rewrite hunion_empty.
-    reflexivity.
-    HDISJ.
-    HDISJ.
-    (* we can't say false if we take the left branch *)
-  Abort.
-
-  Example ex_vacuous_req_wrong : forall x v r, (freq (contains x v)) (hupdate x v hempty) (hempty) false r.
-  Proof.
-    intros.
-    unfold freq.
-    right.
-    (* we can always take the right branch though *)
-    intros.
-    reflexivity.
-  Qed.
-
-  Example ex_vacuous_seq : forall x v r, (freq (contains x v) ;; fens (fun r => contains x v)) (hempty) (hupdate x v hempty) false r.
-  Proof.
-    intros.
-    unfold fseq.
-    right.
-    unfold freq.
-    right.
-    intros.
-    reflexivity.
-  Qed.
-
-  Inductive forward : com -> flow -> Prop :=
-    | fw_skip:
-      forward SKIP fempty
-    | fw_pure: forall n,
-      forward (PURE n) (fens (fun res => pure (res = n)))
-    | fw_get: forall l v, 
-      forward (GET l)
-        (freq (contains l v) ;;
-        (fens (fun r => (r = v) //\\ contains l v)))
-        .
-
-  Definition terminated (c: com) : Prop :=  c = SKIP.
-
-  Definition terminates (c1: com) (h1 h2: heap) : Prop :=
-    exists c2, star red (c1, h1) (c2, h2) /\ terminated c2.
-
-  (* Definition goeswrong (c1: com) (h1: heap) : Prop :=
-    exists c2 h2, star red (c1, h1) (c2, h2) /\ error c2 h2. *)
-
-  (* Fixpoint error (c: com) (s: heap) : Prop :=
-    match c with
-    | ASSERT b => beval b s = false
-    | (c1 ;; c2) => error c1 s
-    | _ => False
-    end. *)
-
-Ltac destr H :=
-  match type of H with
-  | ex _ => 
-    let L := fresh "e" in
-    let R := fresh "H" in
-    destruct H as [L R]; destr R
-  | _ /\ _ => 
-    let L := fresh "L" in
-    let R := fresh "R" in
-    destruct H as [L R]; destr L; destr R
-  | _ => idtac
-  end.
-
-  Theorem soundness : forall c1 h1 h2 h3 r p f,
-    forward c1 f ->
-    terminates c1 h1 h2 ->
-    f h1 h3 p r ->
-    h2 = h3.
-  Proof.
-    (* intros c1. *)
-    (* induction c1; intros. *)
-    intros c1 h1 h2 h3 r p f Hf.
-    induction Hf; intros Hr Hs.
-    -
-      (* skip *)
-    {
-    inv Hr.
-    destruct H.
-    inv H.
-    -
-    (* skip has terminated *)
-      inv H0.
-      unfold fempty in Hs.
-      unfold fens in Hs.
-      destruct Hs as [h0 [H1 [H2 H3]]].
-      subst.
-      rewrite hunion_comm.
-      rewrite -> hunion_empty.
-      auto.
-      rewrite hdisjoint_sym.
-      auto.
-    -
-    (* skip reduces *)
-    inv H1.
-    }
-    -
-    (* pure *)
-    {
-      inv Hr.
-      destruct H. inv H.
-      -
-      (* pure terminates *)
-      unfold fens in Hs.
-      destruct Hs as [h0 [H1 [H2 H3]]].
-      unfold pure in H1.
-      destruct H1.
-      subst.
-      rewrite hunion_comm.
-      rewrite hunion_empty.
-      auto.
-      apply hdisjoint_empty.
-      -
-      (* pure takes steps *)
-      inv H1.
-    }
-    -
-    (* deref *)
-    {
-    inv Hr.
-    destruct H.
-    inv H.
-    -
-    (* get has terminated *)
-    inv H0.
-    - {
-    (* get reduces *)
-    inv H1.
-    inv H2.
-    - {
-    (* pure has terminated *)
-    unfold fseq in Hs.
-    destruct Hs.
-    - {
-      (* seq does not vacuously succeed early *)
-      destr H.
-      unfold freq in L.
-      destr L.
-      destruct L.
-      - destr H. unfold fens in R. destr R. subst.
-      unfold pureconj in L3. destruct L3. subst.
-      unfold contains in H1.
-      unfold contains in L1.
-      subst.
-      rewrite hunion_comm; auto.
-      -
-      pose proof (H h2 h3).
-      destr H1.
-      (* inv R0. *)
+  intros f c1 h1 h2 h3 Hs.
+  induction Hs; intros Hf Ht.
+  - inv Hf.
+  - { inv Hf.
+    - { inv Ht.
       admit.
     }
-    -
-      (* seq vacuously succeeds early *)
-      { inv H0.
-      inv H.
-      destruct H0.
-      destruct H.
-      - destr H. inv R0.
-      - admit.
-      }
-    } 
-    -
-    (* pure reduces *)
-    inv H.
-}
-    }
-  (* Qed. *)
-  Admitted.
+    (* - inv Ht. inv H0. inv H1. inv H2. inv H. inv H1. inv H0. rewrite hunion_comm. rewrite hunion_empty. auto. *)
+    (* HDISJ. inv H0. *)
+    - admit.
+  }
+Admitted.
+(* Qed. *)
 
-End Flow2.
+
+End Flow3.
